Fixed main compile logic, need to remove assumption from Changes Lemma

common.dfy
@@ -111,41 +111,195 @@ module Common{
         else if 0< |p.commands| <= 1 then [0]
         else ChangesHelper(p, 0)
     }
-
-    ghost predicate change_helper_correct(p: Program, i: int, res: seq<int>)
-    requires 0 <= i <= |p.commands|
-    // requires res == ChangesHelper(p, i)
-    {
-        (i == |p.commands| ==> !(i in res)
-        )&&(forall d:: 0<= d <|res| ==> 0<= res[d] <|p.commands|
-        )&&(forall d:: 0 <= d < |res|-1 && p.commands[res[d]] in ['+', '-', '<', '>'] ==> res[d+1]==res[d]+ count_consecutive_symbols(p, res[d])
-        )&&(forall d:: 0<= d <|res|-1 && p.commands[res[d]] in ['+', '-', '<', '>']==> ((p.commands[res[d]]!=p.commands[res[d+1]]))
-        )&&(forall d:: (0<= d <|res|-1 && !(p.commands[res[d]] in ['+', '-', '<', '>']))==> (res[d+1]-res[d] ==1)
-        )&&(forall d:: (d in res && p.commands[d] in ['+', '-', '<', '>']) ==> ((d+count_consecutive_symbols(p, d) >= |p.commands|) || d+count_consecutive_symbols(p, d) in res)
-        )&&(forall d:: (d in res && !(p.commands[d] in ['+', '-', '<', '>'])) ==> ((d+1 >= |p.commands|) || d+1 in res)
-)
-    }
     function  ChangesHelper(p: Program, i: int): seq<int>
         requires 0 <= i <= |p.commands|
         decreases |p.commands|-i 
-        // ensures change_helper_correct(p, i, ChangesHelper(p, i))
-        // ensures i == |p.commands| ==> !(i in ChangesHelper(p, i))
-        // // ensures forall d:: (d in ChangesHelper(p, i) && p.commands[d] in ['+', '-', '<', '>']  && d + count_consecutive_symbols(p, d) < |p.commands|) ==> d+ count_consecutive_symbols(p, d) in ChangesHelper(p, i)
-        // ensures forall d:: 0<= d <|ChangesHelper(p, i)| ==> 0<= ChangesHelper(p, i)[d] <|p.commands|
-        // ensures forall d:: 0 <= d < |ChangesHelper(p, i)|-1 && p.commands[ChangesHelper(p, i)[d]] in ['+', '-', '<', '>'] ==> ChangesHelper(p, i)[d+1]==ChangesHelper(p, i)[d]+ count_consecutive_symbols(p, ChangesHelper(p, i)[d])
-        // // ensures forall d:: 0<= d < |ChangesHelper(p, i)|-1 && p.commands[ChangesHelper(p, i)[d]] in ['+', '-', '<', '>'] ==> ChangesHelper(p, i)[d+1]-ChangesHelper(p, i)[d] == count_consecutive_symbols(p, ChangesHelper(p, i)[d])
-        // ensures forall d:: 0<= d <|ChangesHelper(p, i)|-1 && p.commands[ChangesHelper(p, i)[d]] in ['+', '-', '<', '>']==> ((p.commands[ChangesHelper(p, i)[d]]!=p.commands[ChangesHelper(p, i)[d+1]]))
-        // ensures forall d:: (0<= d <|ChangesHelper(p, i)|-1 && !(p.commands[ChangesHelper(p, i)[d]] in ['+', '-', '<', '>']))==> (ChangesHelper(p, i)[d+1]-ChangesHelper(p, i)[d] ==1)
-        // ensures forall d:: (d in ChangesHelper(p, i) && p.commands[d] in ['+', '-', '<', '>']) ==> ((d+count_consecutive_symbols(p, d) >= |p.commands|) || d+count_consecutive_symbols(p, d) in ChangesHelper(p, i))
-        // ensures forall d:: (d in ChangesHelper(p,i) && !(p.commands[d] in ['+', '-', '<', '>'])) ==> ((d+1 >= |p.commands|) || d+1 in ChangesHelper(p,i))
-
-        // ensures forall d:: 0<=d<|ChangesHelper(s, i)|-1 ==> forall j:: ChangesHelper(s, i)[d] <= j < ChangesHelper(s, i)[d+1] ==> s[j] != s[ChangesHelper(s, i)[d+1]]
-        // ensures matching_pred(s, ChangesHelper(s, i))
     {
         if i == |p.commands| then []
         else if p.commands[i] in ['+', '-', '<', '>'] then [i] + ChangesHelper(p, i + count_consecutive_symbols(p, i))
         else [i]+ ChangesHelper(p, i + 1)
     }    
+    ghost predicate change_helper_correct(p: Program, i: int, res: seq<int>)
+    requires 0 <= i <= |p.commands|
+    // requires res == ChangesHelper(p, i)
+    {
+        (i == |p.commands| ==> !(i in res))
+        &&
+        (i < |p.commands| ==> (
+        (forall d:: 0<= d <|res| ==> 0<= res[d] <|p.commands|)
+        &&
+        (forall d:: 0 <= d < |res|-1 && p.commands[res[d]] in ['+', '-', '<', '>'] ==> (res[d+1]==res[d]+ count_consecutive_symbols(p, res[d]) && ((p.commands[res[d]]!=p.commands[res[d+1]]))))
+        &&
+        (forall d:: (0<= d <|res|-1 && !(p.commands[res[d]] in ['+', '-', '<', '>']))==> (res[d+1]-res[d] ==1))
+        &&
+        (forall d:: (d in res && p.commands[d] in ['+', '-', '<', '>']) ==> ((d+count_consecutive_symbols(p, d) == |p.commands|) || d+count_consecutive_symbols(p, d) in res))
+        &&
+        (forall d:: (d in res && !(p.commands[d] in ['+', '-', '<', '>'])) ==> ((d+1 == |p.commands|) || d+1 in res)
+))
+        )
+    }
+ 
+    lemma StrictlyIncreasingImpliesUnique(s: seq<int>) 
+    requires forall i, j :: 0<= i < j < |s| ==> s[i] < s[j]  // The sequence is strictly increasing
+    ensures forall i, j :: i != j && 0<= i < |s| && 0<= j <|s| ==> s[i] != s[j]
+
+{
+    // Prove that all elements are unique
+}
+    ghost predicate int_in_seq(k: int, s: seq<int>){
+        k in s
+    }
+
+    lemma trivialBiggerNotEq(s: seq<int>, i: int)
+    requires forall k:: k in s ==> i > k
+    ensures forall k:: int_in_seq(k, s) ==> i!= k 
+    {}
+    ghost predicate greater_than_and_in_seq( k: int, i: int, s2: seq<int>){
+        (i> k && k in s2)
+    }
+
+    ghost predicate sub_changes_1_step(p: Program, next_command_indices: seq<int>)
+    requires forall d:: 0<= d < |next_command_indices| ==> 0<=next_command_indices[d]<|p.commands|
+    {
+        forall d :: (0 <= d < |next_command_indices| && !(p.commands[next_command_indices[d]] in ['+', '-', '>', '<'])) ==> next_step(p, next_command_indices[d], 1, next_command_indices)
+    }
+    ghost predicate next_step(p: Program, i: int, k: int, next_command_indices: seq<int>)
+    requires i in next_command_indices
+    {
+        inside_the_indices(p, next_command_indices, i+k)
+    }
+    ghost predicate relation_between_old_new(p: Program, old_i: int, i: int, next_command_indices: seq<int>)
+    {
+        (old_i in next_command_indices) ==> inside_the_indices(p, next_command_indices, i)
+    }
+    lemma simple_exclusion(symb: char)
+    requires symb == '.' 
+    ensures !(symb in ['+', '-', '>', '<'])
+    {}
+
+    lemma simple_exclusion_2(symb: char)
+        requires symb == ',' 
+        ensures !(symb in ['+', '-', '>', '<'])
+    {}
+
+
+    lemma addition_is_preserving(p: Program, old_i: int, i: int, k: int, summation: int, next_command_indices: seq<int>)
+    requires summation == i+k
+    requires relation_between_old_new(p, old_i, i+k, next_command_indices)
+    ensures relation_between_old_new(p, old_i, summation, next_command_indices)
+    {
+        
+    }
+
+    lemma addition_is_preserving_one(p: Program, old_i: int, i: int, summation: int, next_command_indices: seq<int>)
+    requires summation == i+1
+    requires relation_between_old_new(p, old_i, i+1, next_command_indices)
+    ensures relation_between_old_new(p, old_i, summation, next_command_indices)
+    {
+        
+    }
+
+    lemma step_is_indices(p: Program, i: int, k: int, next_command_indices: seq<int>)
+    requires (i in next_command_indices && next_step(p, i, k, next_command_indices)) ==> inside_the_indices(p, next_command_indices, i+k)
+    requires i in next_command_indices ==> next_step(p, i, k, next_command_indices)
+    ensures (i in next_command_indices) ==> inside_the_indices(p, next_command_indices, i+k)
+    {}
+
+    lemma one_step_is_indices(p: Program, i: int, next_command_indices: seq<int>)
+        requires (i in next_command_indices && next_step(p, i, 1, next_command_indices)) ==> inside_the_indices(p, next_command_indices, i+1)
+        requires i in next_command_indices ==> next_step(p, i, 1, next_command_indices)
+        ensures (i in next_command_indices) ==> inside_the_indices(p, next_command_indices, i+1)
+    {}
+
+    lemma implication_with_and(p: Program, i: int, k: int, next_command_indices: seq<int>)
+    ensures (i in next_command_indices && next_step(p, i, k, next_command_indices)) ==> inside_the_indices(p, next_command_indices, i+k)
+    {}
+
+    lemma implication_with_and_2(p: Program, i: int, next_command_indices: seq<int>)
+    requires 0<= i < |p.commands| && !(p.commands[i] in ['+', '-', '>', '<']) 
+    ensures (i in next_command_indices && next_step(p, i, 1, next_command_indices)) ==> inside_the_indices(p, next_command_indices, i+1)
+    {}
+
+    ghost predicate sub_changes(p: Program, next_command_indices: seq<int>)
+    requires forall d:: 0<= d < |next_command_indices| ==> 0<=next_command_indices[d]<|p.commands|
+    {
+        forall d :: (0 <= d < |next_command_indices| && (p.commands[next_command_indices[d]] in ['+', '-', '>', '<'])) ==> next_step(p, next_command_indices[d], count_consecutive_symbols(p, next_command_indices[d]), next_command_indices)
+    }
+
+    predicate inside_the_indices(p: Program, next_command_indices: seq<int>, i: int){
+       (i == |p.commands|) || (i < |p.commands| && i in next_command_indices)
+    }
+
+    ghost predicate sub_changes_inclusion(p: Program, next_command_indices: seq<int>)
+    requires forall d:: 0<= d < |next_command_indices| ==> 0<=next_command_indices[d]<|p.commands|
+    {
+        forall d:: (d in next_command_indices && p.commands[d] in ['+', '-', '<', '>']) ==> next_step(p, d, count_consecutive_symbols(p, d), next_command_indices) 
+
+    }
+    ghost predicate sub_changes_inclusion_1_step(p: Program, next_command_indices: seq<int>)
+    requires forall d:: 0<= d < |next_command_indices| ==> 0<=next_command_indices[d]<|p.commands|
+    {
+        forall d:: (d in next_command_indices && !(p.commands[d] in ['+', '-', '<', '>'])) ==> next_step(p, d, 1, next_command_indices)
+
+    }
+    ghost predicate changes_correct(p: Program, res: seq<int>)
+    {
+        (forall d:: 0<= d < |res| ==>
+            (0 <= res[d] < |p.commands| &&
+            ( 0 <= d < |res|-1 && p.commands[res[d]] in ['+', '-', '>', '<'] ==>(
+                res[d+1] == res[d] + count_consecutive_symbols(p, res[d])
+                && res[d+1] != res[d]
+            )) &&
+            (((p.commands[res[d]] in ['+', '-', '>', '<'])) ==>
+                (res[d]+count_consecutive_symbols(p, res[d]) == |p.commands| || (res[d]+count_consecutive_symbols(p, res[d]) < |p.commands| &&res[d]+count_consecutive_symbols(p, res[d]) in res)))    
+            &&
+            ((0 <= d < |res| && !(p.commands[res[d]] in ['+', '-', '>', '<'])) ==>
+                (res[d]+1 == |p.commands| || (res[d]+1 < |p.commands| && res[d]+1 in res)))    
+            )
+            &&
+            ( 0 <= d < |res|-1 && !(p.commands[res[d]] in ['+', '-', '>', '<']) ==>(
+                res[d+1] == res[d] + 1
+            ))
+        )
+    }
+    lemma zero_implies_all (j: int, s1: seq<int>, s2: seq<int>)
+    requires j==0
+    ensures 1<=j<=|s2| ==> s1[j-1]==s2[j-1]
+    {}
+
+    lemma extension (j: int, s1: seq<int>, s2: seq<int>)
+    requires 0<= j < |s1|
+    requires |s1| == j+1
+    requires j < |s2| ==> s1[j]==s2[j]
+    requires j <= |s2| ==> s1[..j] == s2[..j]
+    ensures j+1 <= |s2| ==> s1 == s2[..j+1]
+    {}
+
+    lemma addition_preserving_2 (s1: seq<int>, s2: seq<int>, j: int, k: int)
+    requires 0<= j < |s1|
+    requires 1<= j+1 <= |s2| ==> s1[j] == s2[j]
+    requires k == j+1
+    ensures 1<= k <= |s2| ==> s2[k-1] == s2[k-1]
+    {}
+
+    lemma addition_preserving_3 (s1: seq<int>, s2: seq<int>, j: int, k: int)
+    requires 0<= j < |s1|
+    requires j+1 <= |s2| ==> s1 == s2[..j+1]
+    requires k == j+1
+    ensures k <= |s2| ==> s1 == s2[..k]
+    {}
+
+
+    lemma isolate_changes_correct(p: Program, res: seq<int>)
+    requires changes_correct(p, res)
+    ensures forall d:: 0<=d < |res| ==>
+        (0 <= res[d] < |p.commands| &&
+            ( 0 <= d < |res|-1 && p.commands[res[d]] in ['+', '-', '>', '<'] ==>(
+                res[d+1] == res[d] + count_consecutive_symbols(p, res[d])
+                && res[d+1] != res[d]
+            ))
+        ) 
+{}
     function count_consecutive_symbols(p: Program, idx: int): nat
         requires 0 <= idx < |p.commands|
         ensures idx + count_consecutive_symbols(p, idx) <= |p.commands|
@@ -158,4 +312,7 @@ module Common{
         else 
             1
     }
+
+
+
 }
